Auto/Embedding/LamInductive.lean
@@ -1,0 +1,18 @@
+import Auto.Embedding.LamConv
+
+namespace Auto.Embedding.Lam
+
+structure IndInfo where
+  type  : LamSort
+  ctors : List (LamSort × LamTerm)
+
+def IndInfo.toString (i : IndInfo) :=
+  s!"IndInfo ⦗⦗ {i.type} || " ++ String.intercalate ", "
+    (i.ctors.map (fun (s, t) => s!"{t} : {s}")) ++ " ⦘⦘"
+
+instance : ToString IndInfo where
+  toString := IndInfo.toString
+
+abbrev MutualIndInfo := List IndInfo
+
+end Auto.Embedding.Lam
