Test/SmtTranslation/Inductive.lean
@@ -1,0 +1,79 @@
+import Auto.Tactic
+
+set_option auto.smt true
+set_option trace.auto.smt.printCommands true
+set_option trace.auto.smt.result true
+set_option auto.proofReconstruction false
+
+section Enum
+
+  example (x y : Unit) : x = y := by auto
+
+  -- **TODO**:
+  -- SMT solver does not understand empty type,
+  -- This can be fixed by translating `∀ x : Empty` as `True`, `∃ x : Empty` as `False`, and any `fvar : Empty` as `False`
+  example (x y : Empty) : x = y := by auto
+
+  private inductive Color where
+    | red
+    | green
+    | ultraviolet
+
+  example (x y z t : Color) : x = y ∨ x = z ∨ x = t ∨ y = z ∨ y = t ∨ z = t := by auto
+
+end Enum
+
+section NonRecursive
+
+  -- **TODO**:
+  -- · Recognize projections for structures
+  -- · Better control over input??
+  set_option trace.auto.lamReif.printResult true
+  example (x : α × β) : x = (Prod.fst x, Prod.snd x) := by
+    have h₁ : ∀ (x : α) (y : β) (z : α × β), z = (x, y) → Prod.fst z = x := fun _ _ _ h => by cases h; rfl
+    have h₁ : ∀ (x : α) (y : β) (z : α × β), z = (x, y) → Prod.snd z = y := fun _ _ _ h => by cases h; rfl
+    auto
+
+end NonRecursive
+
+section Recursive
+
+  -- SMT solver is now able to recognize inductive types
+  set_option auto.lamReif.prep.def false
+  set_option trace.auto.lamReif.printResult true
+  example (x y : α) : [x] ++ [y] = [x, y] := by
+    -- Invoke definition unfolding
+    -- **TODO**: Apply unfolding to λ inductive infos
+    have h : ∀ (x y : List α), x ++ y = x.append y := fun _ _ => rfl
+    auto [h] d[List.append]
+
+  -- SMT solver times out on the following problem:
+  -- set_option auto.prep.redMode "all" in
+  -- example (x y z : List Nat) : (x ++ y) ++ z = x ++ (y ++ z) := by
+  --   auto d[List.append]
+
+  mutual
+
+    private inductive tree where
+      | leaf : Nat → tree
+      | node : treelist → tree
+
+    private inductive treelist where
+      | nil : treelist
+      | cons : tree → treelist → treelist
+
+  end
+
+  set_option trace.auto.lamReif.printResult true
+  example (x : tree) : (∃ (y : treelist), x = .node y) ∨ (∃ y, x = .leaf y) := by
+    auto
+
+end Recursive
+
+/- Issues to be solved:
+  1. Unable to deal with inductive families, like `Vector`
+  2. Fails if constructor is dependent/polymorphic after monomorphization,
+     for example `Fin`
+  3. Change `leaf : Nat → tree` into `leaf : Unit → Tree`,
+     and `(∃ y, x = .leaf y)` into `x = ()`, the above example will fail
+-/
